hax-lib/proof-libs/fstar/core/Core_models.Iter.Ends.fst
@@ -4,505 +4,103 @@ open FStar.Mul
 open Rust_primitives
 
 [@@ FStar.Tactics.Typeclasses.tcinstance]
-let impl_2: Core_models.Iter.Traits.Double_ended.t_DoubleEndedIterator
-(Core_models.Ops.Range.t_Range u8) =
-  {
-    _super_i0 = FStar.Tactics.Typeclasses.solve;
-    f_next_back_pre = (fun (self: Core_models.Ops.Range.t_Range u8) -> true);
-    f_next_back_post
-    =
-    (fun
-        (self: Core_models.Ops.Range.t_Range u8)
-        (out: (Core_models.Ops.Range.t_Range u8 & Core_models.Option.t_Option u8))
-        ->
-        true);
-    f_next_back
-    =
-    fun (self: Core_models.Ops.Range.t_Range u8) ->
-      let
-      (self: Core_models.Ops.Range.t_Range u8), (hax_temp_output: Core_models.Option.t_Option u8) =
-        if self.Core_models.Ops.Range.f_start >=. self.Core_models.Ops.Range.f_end
-        then
-          self, (Core_models.Option.Option_None <: Core_models.Option.t_Option u8)
-          <:
-          (Core_models.Ops.Range.t_Range u8 & Core_models.Option.t_Option u8)
-        else
-          let self:Core_models.Ops.Range.t_Range u8 =
-            { self with Core_models.Ops.Range.f_end = self.Core_models.Ops.Range.f_end -! mk_u8 1 }
-            <:
-            Core_models.Ops.Range.t_Range u8
-          in
-          self,
-          (Core_models.Option.Option_Some self.Core_models.Ops.Range.f_end
-            <:
-            Core_models.Option.t_Option u8)
-          <:
-          (Core_models.Ops.Range.t_Range u8 & Core_models.Option.t_Option u8)
-      in
-      self, hax_temp_output <: (Core_models.Ops.Range.t_Range u8 & Core_models.Option.t_Option u8)
-  }
+assume
+val impl_1': Core_models.Iter.Traits.Double_ended.t_DoubleEndedIterator
+(Core_models.Ops.Range.t_Range u8)
+
+unfold
+let impl_1 = impl_1'
 
 [@@ FStar.Tactics.Typeclasses.tcinstance]
-let impl_3: Core_models.Iter.Traits.Double_ended.t_DoubleEndedIterator
-(Core_models.Ops.Range.t_Range u16) =
-  {
-    _super_i0 = FStar.Tactics.Typeclasses.solve;
-    f_next_back_pre = (fun (self: Core_models.Ops.Range.t_Range u16) -> true);
-    f_next_back_post
-    =
-    (fun
-        (self: Core_models.Ops.Range.t_Range u16)
-        (out: (Core_models.Ops.Range.t_Range u16 & Core_models.Option.t_Option u16))
-        ->
-        true);
-    f_next_back
-    =
-    fun (self: Core_models.Ops.Range.t_Range u16) ->
-      let
-      (self: Core_models.Ops.Range.t_Range u16), (hax_temp_output: Core_models.Option.t_Option u16)
-      =
-        if self.Core_models.Ops.Range.f_start >=. self.Core_models.Ops.Range.f_end
-        then
-          self, (Core_models.Option.Option_None <: Core_models.Option.t_Option u16)
-          <:
-          (Core_models.Ops.Range.t_Range u16 & Core_models.Option.t_Option u16)
-        else
-          let self:Core_models.Ops.Range.t_Range u16 =
-            { self with Core_models.Ops.Range.f_end = self.Core_models.Ops.Range.f_end -! mk_u16 1 }
-            <:
-            Core_models.Ops.Range.t_Range u16
-          in
-          self,
-          (Core_models.Option.Option_Some self.Core_models.Ops.Range.f_end
-            <:
-            Core_models.Option.t_Option u16)
-          <:
-          (Core_models.Ops.Range.t_Range u16 & Core_models.Option.t_Option u16)
-      in
-      self, hax_temp_output <: (Core_models.Ops.Range.t_Range u16 & Core_models.Option.t_Option u16)
-  }
+assume
+val impl_2': Core_models.Iter.Traits.Double_ended.t_DoubleEndedIterator
+(Core_models.Ops.Range.t_Range u16)
+
+unfold
+let impl_2 = impl_2'
 
 [@@ FStar.Tactics.Typeclasses.tcinstance]
-let impl_4: Core_models.Iter.Traits.Double_ended.t_DoubleEndedIterator
-(Core_models.Ops.Range.t_Range u32) =
-  {
-    _super_i0 = FStar.Tactics.Typeclasses.solve;
-    f_next_back_pre = (fun (self: Core_models.Ops.Range.t_Range u32) -> true);
-    f_next_back_post
-    =
-    (fun
-        (self: Core_models.Ops.Range.t_Range u32)
-        (out: (Core_models.Ops.Range.t_Range u32 & Core_models.Option.t_Option u32))
-        ->
-        true);
-    f_next_back
-    =
-    fun (self: Core_models.Ops.Range.t_Range u32) ->
-      let
-      (self: Core_models.Ops.Range.t_Range u32), (hax_temp_output: Core_models.Option.t_Option u32)
-      =
-        if self.Core_models.Ops.Range.f_start >=. self.Core_models.Ops.Range.f_end
-        then
-          self, (Core_models.Option.Option_None <: Core_models.Option.t_Option u32)
-          <:
-          (Core_models.Ops.Range.t_Range u32 & Core_models.Option.t_Option u32)
-        else
-          let self:Core_models.Ops.Range.t_Range u32 =
-            { self with Core_models.Ops.Range.f_end = self.Core_models.Ops.Range.f_end -! mk_u32 1 }
-            <:
-            Core_models.Ops.Range.t_Range u32
-          in
-          self,
-          (Core_models.Option.Option_Some self.Core_models.Ops.Range.f_end
-            <:
-            Core_models.Option.t_Option u32)
-          <:
-          (Core_models.Ops.Range.t_Range u32 & Core_models.Option.t_Option u32)
-      in
-      self, hax_temp_output <: (Core_models.Ops.Range.t_Range u32 & Core_models.Option.t_Option u32)
-  }
+assume
+val impl_3': Core_models.Iter.Traits.Double_ended.t_DoubleEndedIterator
+(Core_models.Ops.Range.t_Range u32)
+
+unfold
+let impl_3 = impl_3'
 
 [@@ FStar.Tactics.Typeclasses.tcinstance]
-let impl_5: Core_models.Iter.Traits.Double_ended.t_DoubleEndedIterator
-(Core_models.Ops.Range.t_Range u64) =
-  {
-    _super_i0 = FStar.Tactics.Typeclasses.solve;
-    f_next_back_pre = (fun (self: Core_models.Ops.Range.t_Range u64) -> true);
-    f_next_back_post
-    =
-    (fun
-        (self: Core_models.Ops.Range.t_Range u64)
-        (out: (Core_models.Ops.Range.t_Range u64 & Core_models.Option.t_Option u64))
-        ->
-        true);
-    f_next_back
-    =
-    fun (self: Core_models.Ops.Range.t_Range u64) ->
-      let
-      (self: Core_models.Ops.Range.t_Range u64), (hax_temp_output: Core_models.Option.t_Option u64)
-      =
-        if self.Core_models.Ops.Range.f_start >=. self.Core_models.Ops.Range.f_end
-        then
-          self, (Core_models.Option.Option_None <: Core_models.Option.t_Option u64)
-          <:
-          (Core_models.Ops.Range.t_Range u64 & Core_models.Option.t_Option u64)
-        else
-          let self:Core_models.Ops.Range.t_Range u64 =
-            { self with Core_models.Ops.Range.f_end = self.Core_models.Ops.Range.f_end -! mk_u64 1 }
-            <:
-            Core_models.Ops.Range.t_Range u64
-          in
-          self,
-          (Core_models.Option.Option_Some self.Core_models.Ops.Range.f_end
-            <:
-            Core_models.Option.t_Option u64)
-          <:
-          (Core_models.Ops.Range.t_Range u64 & Core_models.Option.t_Option u64)
-      in
-      self, hax_temp_output <: (Core_models.Ops.Range.t_Range u64 & Core_models.Option.t_Option u64)
-  }
+assume
+val impl_4': Core_models.Iter.Traits.Double_ended.t_DoubleEndedIterator
+(Core_models.Ops.Range.t_Range u64)
+
+unfold
+let impl_4 = impl_4'
 
 [@@ FStar.Tactics.Typeclasses.tcinstance]
-let impl_6: Core_models.Iter.Traits.Double_ended.t_DoubleEndedIterator
-(Core_models.Ops.Range.t_Range u128) =
-  {
-    _super_i0 = FStar.Tactics.Typeclasses.solve;
-    f_next_back_pre = (fun (self: Core_models.Ops.Range.t_Range u128) -> true);
-    f_next_back_post
-    =
-    (fun
-        (self: Core_models.Ops.Range.t_Range u128)
-        (out: (Core_models.Ops.Range.t_Range u128 & Core_models.Option.t_Option u128))
-        ->
-        true);
-    f_next_back
-    =
-    fun (self: Core_models.Ops.Range.t_Range u128) ->
-      let
-      (self: Core_models.Ops.Range.t_Range u128),
-      (hax_temp_output: Core_models.Option.t_Option u128) =
-        if self.Core_models.Ops.Range.f_start >=. self.Core_models.Ops.Range.f_end
-        then
-          self, (Core_models.Option.Option_None <: Core_models.Option.t_Option u128)
-          <:
-          (Core_models.Ops.Range.t_Range u128 & Core_models.Option.t_Option u128)
-        else
-          let self:Core_models.Ops.Range.t_Range u128 =
-            {
-              self with
-              Core_models.Ops.Range.f_end = self.Core_models.Ops.Range.f_end -! mk_u128 1
-            }
-            <:
-            Core_models.Ops.Range.t_Range u128
-          in
-          self,
-          (Core_models.Option.Option_Some self.Core_models.Ops.Range.f_end
-            <:
-            Core_models.Option.t_Option u128)
-          <:
-          (Core_models.Ops.Range.t_Range u128 & Core_models.Option.t_Option u128)
-      in
-      self, hax_temp_output
-      <:
-      (Core_models.Ops.Range.t_Range u128 & Core_models.Option.t_Option u128)
-  }
+assume
+val impl_5': Core_models.Iter.Traits.Double_ended.t_DoubleEndedIterator
+(Core_models.Ops.Range.t_Range u128)
+
+unfold
+let impl_5 = impl_5'
 
 [@@ FStar.Tactics.Typeclasses.tcinstance]
-let impl_7: Core_models.Iter.Traits.Double_ended.t_DoubleEndedIterator
-(Core_models.Ops.Range.t_Range usize) =
-  {
-    _super_i0 = FStar.Tactics.Typeclasses.solve;
-    f_next_back_pre = (fun (self: Core_models.Ops.Range.t_Range usize) -> true);
-    f_next_back_post
-    =
-    (fun
-        (self: Core_models.Ops.Range.t_Range usize)
-        (out: (Core_models.Ops.Range.t_Range usize & Core_models.Option.t_Option usize))
-        ->
-        true);
-    f_next_back
-    =
-    fun (self: Core_models.Ops.Range.t_Range usize) ->
-      let
-      (self: Core_models.Ops.Range.t_Range usize),
-      (hax_temp_output: Core_models.Option.t_Option usize) =
-        if self.Core_models.Ops.Range.f_start >=. self.Core_models.Ops.Range.f_end
-        then
-          self, (Core_models.Option.Option_None <: Core_models.Option.t_Option usize)
-          <:
-          (Core_models.Ops.Range.t_Range usize & Core_models.Option.t_Option usize)
-        else
-          let self:Core_models.Ops.Range.t_Range usize =
-            {
-              self with
-              Core_models.Ops.Range.f_end = self.Core_models.Ops.Range.f_end -! mk_usize 1
-            }
-            <:
-            Core_models.Ops.Range.t_Range usize
-          in
-          self,
-          (Core_models.Option.Option_Some self.Core_models.Ops.Range.f_end
-            <:
-            Core_models.Option.t_Option usize)
-          <:
-          (Core_models.Ops.Range.t_Range usize & Core_models.Option.t_Option usize)
-      in
-      self, hax_temp_output
-      <:
-      (Core_models.Ops.Range.t_Range usize & Core_models.Option.t_Option usize)
-  }
+assume
+val impl_6': Core_models.Iter.Traits.Double_ended.t_DoubleEndedIterator
+(Core_models.Ops.Range.t_Range usize)
+
+unfold
+let impl_6 = impl_6'
 
 [@@ FStar.Tactics.Typeclasses.tcinstance]
-let impl_8: Core_models.Iter.Traits.Double_ended.t_DoubleEndedIterator
-(Core_models.Ops.Range.t_Range i8) =
-  {
-    _super_i0 = FStar.Tactics.Typeclasses.solve;
-    f_next_back_pre = (fun (self: Core_models.Ops.Range.t_Range i8) -> true);
-    f_next_back_post
-    =
-    (fun
-        (self: Core_models.Ops.Range.t_Range i8)
-        (out: (Core_models.Ops.Range.t_Range i8 & Core_models.Option.t_Option i8))
-        ->
-        true);
-    f_next_back
-    =
-    fun (self: Core_models.Ops.Range.t_Range i8) ->
-      let
-      (self: Core_models.Ops.Range.t_Range i8), (hax_temp_output: Core_models.Option.t_Option i8) =
-        if self.Core_models.Ops.Range.f_start >=. self.Core_models.Ops.Range.f_end
-        then
-          self, (Core_models.Option.Option_None <: Core_models.Option.t_Option i8)
-          <:
-          (Core_models.Ops.Range.t_Range i8 & Core_models.Option.t_Option i8)
-        else
-          let self:Core_models.Ops.Range.t_Range i8 =
-            { self with Core_models.Ops.Range.f_end = self.Core_models.Ops.Range.f_end -! mk_i8 1 }
-            <:
-            Core_models.Ops.Range.t_Range i8
-          in
-          self,
-          (Core_models.Option.Option_Some self.Core_models.Ops.Range.f_end
-            <:
-            Core_models.Option.t_Option i8)
-          <:
-          (Core_models.Ops.Range.t_Range i8 & Core_models.Option.t_Option i8)
-      in
-      self, hax_temp_output <: (Core_models.Ops.Range.t_Range i8 & Core_models.Option.t_Option i8)
-  }
+assume
+val impl_7': Core_models.Iter.Traits.Double_ended.t_DoubleEndedIterator
+(Core_models.Ops.Range.t_Range i8)
+
+unfold
+let impl_7 = impl_7'
 
 [@@ FStar.Tactics.Typeclasses.tcinstance]
-let impl_9: Core_models.Iter.Traits.Double_ended.t_DoubleEndedIterator
-(Core_models.Ops.Range.t_Range i16) =
-  {
-    _super_i0 = FStar.Tactics.Typeclasses.solve;
-    f_next_back_pre = (fun (self: Core_models.Ops.Range.t_Range i16) -> true);
-    f_next_back_post
-    =
-    (fun
-        (self: Core_models.Ops.Range.t_Range i16)
-        (out: (Core_models.Ops.Range.t_Range i16 & Core_models.Option.t_Option i16))
-        ->
-        true);
-    f_next_back
-    =
-    fun (self: Core_models.Ops.Range.t_Range i16) ->
-      let
-      (self: Core_models.Ops.Range.t_Range i16), (hax_temp_output: Core_models.Option.t_Option i16)
-      =
-        if self.Core_models.Ops.Range.f_start >=. self.Core_models.Ops.Range.f_end
-        then
-          self, (Core_models.Option.Option_None <: Core_models.Option.t_Option i16)
-          <:
-          (Core_models.Ops.Range.t_Range i16 & Core_models.Option.t_Option i16)
-        else
-          let self:Core_models.Ops.Range.t_Range i16 =
-            { self with Core_models.Ops.Range.f_end = self.Core_models.Ops.Range.f_end -! mk_i16 1 }
-            <:
-            Core_models.Ops.Range.t_Range i16
-          in
-          self,
-          (Core_models.Option.Option_Some self.Core_models.Ops.Range.f_end
-            <:
-            Core_models.Option.t_Option i16)
-          <:
-          (Core_models.Ops.Range.t_Range i16 & Core_models.Option.t_Option i16)
-      in
-      self, hax_temp_output <: (Core_models.Ops.Range.t_Range i16 & Core_models.Option.t_Option i16)
-  }
+assume
+val impl_8': Core_models.Iter.Traits.Double_ended.t_DoubleEndedIterator
+(Core_models.Ops.Range.t_Range i16)
+
+unfold
+let impl_8 = impl_8'
 
 [@@ FStar.Tactics.Typeclasses.tcinstance]
-let impl_10: Core_models.Iter.Traits.Double_ended.t_DoubleEndedIterator
-(Core_models.Ops.Range.t_Range i32) =
-  {
-    _super_i0 = FStar.Tactics.Typeclasses.solve;
-    f_next_back_pre = (fun (self: Core_models.Ops.Range.t_Range i32) -> true);
-    f_next_back_post
-    =
-    (fun
-        (self: Core_models.Ops.Range.t_Range i32)
-        (out: (Core_models.Ops.Range.t_Range i32 & Core_models.Option.t_Option i32))
-        ->
-        true);
-    f_next_back
-    =
-    fun (self: Core_models.Ops.Range.t_Range i32) ->
-      let
-      (self: Core_models.Ops.Range.t_Range i32), (hax_temp_output: Core_models.Option.t_Option i32)
-      =
-        if self.Core_models.Ops.Range.f_start >=. self.Core_models.Ops.Range.f_end
-        then
-          self, (Core_models.Option.Option_None <: Core_models.Option.t_Option i32)
-          <:
-          (Core_models.Ops.Range.t_Range i32 & Core_models.Option.t_Option i32)
-        else
-          let self:Core_models.Ops.Range.t_Range i32 =
-            { self with Core_models.Ops.Range.f_end = self.Core_models.Ops.Range.f_end -! mk_i32 1 }
-            <:
-            Core_models.Ops.Range.t_Range i32
-          in
-          self,
-          (Core_models.Option.Option_Some self.Core_models.Ops.Range.f_end
-            <:
-            Core_models.Option.t_Option i32)
-          <:
-          (Core_models.Ops.Range.t_Range i32 & Core_models.Option.t_Option i32)
-      in
-      self, hax_temp_output <: (Core_models.Ops.Range.t_Range i32 & Core_models.Option.t_Option i32)
-  }
+assume
+val impl_9': Core_models.Iter.Traits.Double_ended.t_DoubleEndedIterator
+(Core_models.Ops.Range.t_Range i32)
+
+unfold
+let impl_9 = impl_9'
 
 [@@ FStar.Tactics.Typeclasses.tcinstance]
-let impl_11: Core_models.Iter.Traits.Double_ended.t_DoubleEndedIterator
-(Core_models.Ops.Range.t_Range i64) =
-  {
-    _super_i0 = FStar.Tactics.Typeclasses.solve;
-    f_next_back_pre = (fun (self: Core_models.Ops.Range.t_Range i64) -> true);
-    f_next_back_post
-    =
-    (fun
-        (self: Core_models.Ops.Range.t_Range i64)
-        (out: (Core_models.Ops.Range.t_Range i64 & Core_models.Option.t_Option i64))
-        ->
-        true);
-    f_next_back
-    =
-    fun (self: Core_models.Ops.Range.t_Range i64) ->
-      let
-      (self: Core_models.Ops.Range.t_Range i64), (hax_temp_output: Core_models.Option.t_Option i64)
-      =
-        if self.Core_models.Ops.Range.f_start >=. self.Core_models.Ops.Range.f_end
-        then
-          self, (Core_models.Option.Option_None <: Core_models.Option.t_Option i64)
-          <:
-          (Core_models.Ops.Range.t_Range i64 & Core_models.Option.t_Option i64)
-        else
-          let self:Core_models.Ops.Range.t_Range i64 =
-            { self with Core_models.Ops.Range.f_end = self.Core_models.Ops.Range.f_end -! mk_i64 1 }
-            <:
-            Core_models.Ops.Range.t_Range i64
-          in
-          self,
-          (Core_models.Option.Option_Some self.Core_models.Ops.Range.f_end
-            <:
-            Core_models.Option.t_Option i64)
-          <:
-          (Core_models.Ops.Range.t_Range i64 & Core_models.Option.t_Option i64)
-      in
-      self, hax_temp_output <: (Core_models.Ops.Range.t_Range i64 & Core_models.Option.t_Option i64)
-  }
+assume
+val impl_10': Core_models.Iter.Traits.Double_ended.t_DoubleEndedIterator
+(Core_models.Ops.Range.t_Range i64)
+
+unfold
+let impl_10 = impl_10'
 
 [@@ FStar.Tactics.Typeclasses.tcinstance]
-let impl_12: Core_models.Iter.Traits.Double_ended.t_DoubleEndedIterator
-(Core_models.Ops.Range.t_Range i128) =
-  {
-    _super_i0 = FStar.Tactics.Typeclasses.solve;
-    f_next_back_pre = (fun (self: Core_models.Ops.Range.t_Range i128) -> true);
-    f_next_back_post
-    =
-    (fun
-        (self: Core_models.Ops.Range.t_Range i128)
-        (out: (Core_models.Ops.Range.t_Range i128 & Core_models.Option.t_Option i128))
-        ->
-        true);
-    f_next_back
-    =
-    fun (self: Core_models.Ops.Range.t_Range i128) ->
-      let
-      (self: Core_models.Ops.Range.t_Range i128),
-      (hax_temp_output: Core_models.Option.t_Option i128) =
-        if self.Core_models.Ops.Range.f_start >=. self.Core_models.Ops.Range.f_end
-        then
-          self, (Core_models.Option.Option_None <: Core_models.Option.t_Option i128)
-          <:
-          (Core_models.Ops.Range.t_Range i128 & Core_models.Option.t_Option i128)
-        else
-          let self:Core_models.Ops.Range.t_Range i128 =
-            {
-              self with
-              Core_models.Ops.Range.f_end = self.Core_models.Ops.Range.f_end -! mk_i128 1
-            }
-            <:
-            Core_models.Ops.Range.t_Range i128
-          in
-          self,
-          (Core_models.Option.Option_Some self.Core_models.Ops.Range.f_end
-            <:
-            Core_models.Option.t_Option i128)
-          <:
-          (Core_models.Ops.Range.t_Range i128 & Core_models.Option.t_Option i128)
-      in
-      self, hax_temp_output
-      <:
-      (Core_models.Ops.Range.t_Range i128 & Core_models.Option.t_Option i128)
-  }
+assume
+val impl_11': Core_models.Iter.Traits.Double_ended.t_DoubleEndedIterator
+(Core_models.Ops.Range.t_Range i128)
+
+unfold
+let impl_11 = impl_11'
 
 [@@ FStar.Tactics.Typeclasses.tcinstance]
-let impl_13: Core_models.Iter.Traits.Double_ended.t_DoubleEndedIterator
-(Core_models.Ops.Range.t_Range isize) =
-  {
-    _super_i0 = FStar.Tactics.Typeclasses.solve;
-    f_next_back_pre = (fun (self: Core_models.Ops.Range.t_Range isize) -> true);
-    f_next_back_post
-    =
-    (fun
-        (self: Core_models.Ops.Range.t_Range isize)
-        (out: (Core_models.Ops.Range.t_Range isize & Core_models.Option.t_Option isize))
-        ->
-        true);
-    f_next_back
-    =
-    fun (self: Core_models.Ops.Range.t_Range isize) ->
-      let
-      (self: Core_models.Ops.Range.t_Range isize),
-      (hax_temp_output: Core_models.Option.t_Option isize) =
-        if self.Core_models.Ops.Range.f_start >=. self.Core_models.Ops.Range.f_end
-        then
-          self, (Core_models.Option.Option_None <: Core_models.Option.t_Option isize)
-          <:
-          (Core_models.Ops.Range.t_Range isize & Core_models.Option.t_Option isize)
-        else
-          let self:Core_models.Ops.Range.t_Range isize =
-            {
-              self with
-              Core_models.Ops.Range.f_end = self.Core_models.Ops.Range.f_end -! mk_isize 1
-            }
-            <:
-            Core_models.Ops.Range.t_Range isize
-          in
-          self,
-          (Core_models.Option.Option_Some self.Core_models.Ops.Range.f_end
-            <:
-            Core_models.Option.t_Option isize)
-          <:
-          (Core_models.Ops.Range.t_Range isize & Core_models.Option.t_Option isize)
-      in
-      self, hax_temp_output
-      <:
-      (Core_models.Ops.Range.t_Range isize & Core_models.Option.t_Option isize)
-  }
+assume
+val impl_12': Core_models.Iter.Traits.Double_ended.t_DoubleEndedIterator
+(Core_models.Ops.Range.t_Range isize)
+
+unfold
+let impl_12 = impl_12'
 
 [@@ FStar.Tactics.Typeclasses.tcinstance]
-let impl_14: Core_models.Iter.Traits.Exact_size.t_ExactSizeIterator
+let impl_13: Core_models.Iter.Traits.Exact_size.t_ExactSizeIterator
 (Core_models.Ops.Range.t_Range u8) =
   {
     _super_i0 = FStar.Tactics.Typeclasses.solve;
@@ -518,7 +116,7 @@ let impl_14: Core_models.Iter.Traits.Exact_size.t_ExactSizeIterator
   }
 
 [@@ FStar.Tactics.Typeclasses.tcinstance]
-let impl_15: Core_models.Iter.Traits.Exact_size.t_ExactSizeIterator
+let impl_14: Core_models.Iter.Traits.Exact_size.t_ExactSizeIterator
 (Core_models.Ops.Range.t_Range u16) =
   {
     _super_i0 = FStar.Tactics.Typeclasses.solve;
@@ -536,7 +134,7 @@ let impl_15: Core_models.Iter.Traits.Exact_size.t_ExactSizeIterator
   }
 
 [@@ FStar.Tactics.Typeclasses.tcinstance]
-let impl_16: Core_models.Iter.Traits.Exact_size.t_ExactSizeIterator
+let impl_15: Core_models.Iter.Traits.Exact_size.t_ExactSizeIterator
 (Core_models.Ops.Range.t_Range u32) =
   {
     _super_i0 = FStar.Tactics.Typeclasses.solve;
@@ -554,7 +152,7 @@ let impl_16: Core_models.Iter.Traits.Exact_size.t_ExactSizeIterator
   }
 
 [@@ FStar.Tactics.Typeclasses.tcinstance]
-let impl_17: Core_models.Iter.Traits.Exact_size.t_ExactSizeIterator
+let impl_16: Core_models.Iter.Traits.Exact_size.t_ExactSizeIterator
 (Core_models.Ops.Range.t_Range usize) =
   {
     _super_i0 = FStar.Tactics.Typeclasses.solve;
@@ -569,7 +167,7 @@ let impl_17: Core_models.Iter.Traits.Exact_size.t_ExactSizeIterator
   }
 
 [@@ FStar.Tactics.Typeclasses.tcinstance]
-let impl_18: Core_models.Iter.Traits.Exact_size.t_ExactSizeIterator
+let impl_17: Core_models.Iter.Traits.Exact_size.t_ExactSizeIterator
 (Core_models.Ops.Range.t_Range i8) =
   {
     _super_i0 = FStar.Tactics.Typeclasses.solve;
@@ -593,7 +191,7 @@ let impl_18: Core_models.Iter.Traits.Exact_size.t_ExactSizeIterator
   }
 
 [@@ FStar.Tactics.Typeclasses.tcinstance]
-let impl_19: Core_models.Iter.Traits.Exact_size.t_ExactSizeIterator
+let impl_18: Core_models.Iter.Traits.Exact_size.t_ExactSizeIterator
 (Core_models.Ops.Range.t_Range i16) =
   {
     _super_i0 = FStar.Tactics.Typeclasses.solve;
@@ -618,7 +216,7 @@ let impl_19: Core_models.Iter.Traits.Exact_size.t_ExactSizeIterator
   }
 
 [@@ FStar.Tactics.Typeclasses.tcinstance]
-let impl_20: Core_models.Iter.Traits.Exact_size.t_ExactSizeIterator
+let impl_19: Core_models.Iter.Traits.Exact_size.t_ExactSizeIterator
 (Core_models.Ops.Range.t_Range i32) =
   {
     _super_i0 = FStar.Tactics.Typeclasses.solve;
@@ -643,7 +241,7 @@ let impl_20: Core_models.Iter.Traits.Exact_size.t_ExactSizeIterator
   }
 
 [@@ FStar.Tactics.Typeclasses.tcinstance]
-let impl_21: Core_models.Iter.Traits.Exact_size.t_ExactSizeIterator
+let impl_20: Core_models.Iter.Traits.Exact_size.t_ExactSizeIterator
 (Core_models.Ops.Range.t_Range isize) =
   {
     _super_i0 = FStar.Tactics.Typeclasses.solve;
@@ -664,48 +262,15 @@ let impl_21: Core_models.Iter.Traits.Exact_size.t_ExactSizeIterator
   }
 
 [@@ FStar.Tactics.Typeclasses.tcinstance]
-let impl (#v_T: Type0)
-    : Core_models.Iter.Traits.Double_ended.t_DoubleEndedIterator (Core_models.Slice.Iter.t_Iter v_T) =
-  {
-    _super_i0 = FStar.Tactics.Typeclasses.solve;
-    f_next_back_pre = (fun (self: Core_models.Slice.Iter.t_Iter v_T) -> true);
-    f_next_back_post
-    =
-    (fun
-        (self: Core_models.Slice.Iter.t_Iter v_T)
-        (out1: (Core_models.Slice.Iter.t_Iter v_T & Core_models.Option.t_Option v_T))
-        ->
-        true);
-    f_next_back
-    =
-    fun (self: Core_models.Slice.Iter.t_Iter v_T) ->
-      let n:usize = Rust_primitives.Sequence.seq_len #v_T self.Core_models.Slice.Iter._0 in
-      let
-      (self: Core_models.Slice.Iter.t_Iter v_T), (hax_temp_output: Core_models.Option.t_Option v_T)
-      =
-        if n =. mk_usize 0
-        then
-          self, (Core_models.Option.Option_None <: Core_models.Option.t_Option v_T)
-          <:
-          (Core_models.Slice.Iter.t_Iter v_T & Core_models.Option.t_Option v_T)
-        else
-          let (tmp0: Rust_primitives.Sequence.t_Seq v_T), (out: v_T) =
-            Rust_primitives.Sequence.seq_remove #v_T
-              self.Core_models.Slice.Iter._0
-              (n -! mk_usize 1 <: usize)
-          in
-          let self:Core_models.Slice.Iter.t_Iter v_T =
-            { self with Core_models.Slice.Iter._0 = tmp0 } <: Core_models.Slice.Iter.t_Iter v_T
-          in
-          self, (Core_models.Option.Option_Some out <: Core_models.Option.t_Option v_T)
-          <:
-          (Core_models.Slice.Iter.t_Iter v_T & Core_models.Option.t_Option v_T)
-      in
-      self, hax_temp_output <: (Core_models.Slice.Iter.t_Iter v_T & Core_models.Option.t_Option v_T)
-  }
+assume
+val impl_21': #v_T: Type0
+  -> Core_models.Iter.Traits.Double_ended.t_DoubleEndedIterator (Core_models.Slice.Iter.t_Iter v_T)
+
+unfold
+let impl_21 (#v_T: Type0) = impl_21' #v_T
 
 [@@ FStar.Tactics.Typeclasses.tcinstance]
-let impl_1 (#v_T: Type0)
+let impl (#v_T: Type0)
     : Core_models.Iter.Traits.Exact_size.t_ExactSizeIterator (Core_models.Slice.Iter.t_Iter v_T) =
   {
     _super_i0 = FStar.Tactics.Typeclasses.solve;
