hax-lib/proof-libs/fstar/core/Core_models.Iter.Sources.Once_with.fst
@@ -17,44 +17,19 @@ let once_with
     : t_OnceWith v_F = OnceWith (Rust_primitives.Sequence.seq_one #v_F make) <: t_OnceWith v_F
 
 [@@ FStar.Tactics.Typeclasses.tcinstance]
+assume
+val impl':
+    #v_A: Type0 ->
+    #v_F: Type0 ->
+    {| i0: Core_models.Ops.Function.t_FnOnce v_F Prims.unit |} ->
+    #_: unit{i0.Core_models.Ops.Function.f_Output == v_A}
+  -> Core_models.Iter.Traits.Iterator.t_Iterator (t_OnceWith v_F)
+
+unfold
 let impl
       (#v_A #v_F: Type0)
       (#[FStar.Tactics.Typeclasses.tcresolve ()]
           i0:
           Core_models.Ops.Function.t_FnOnce v_F Prims.unit)
       (#_: unit{i0.Core_models.Ops.Function.f_Output == v_A})
-    : Core_models.Iter.Traits.Iterator.t_Iterator (t_OnceWith v_F) =
-  {
-    f_Item = v_A;
-    f_next_pre = (fun (self: t_OnceWith v_F) -> true);
-    f_next_post
-    =
-    (fun (self: t_OnceWith v_F) (out1: (t_OnceWith v_F & Core_models.Option.t_Option v_A)) -> true);
-    f_next
-    =
-    fun (self: t_OnceWith v_F) ->
-      let (self: t_OnceWith v_F), (hax_temp_output: Core_models.Option.t_Option v_A) =
-        if (Rust_primitives.Sequence.seq_len #v_F self._0 <: usize) =. mk_usize 0
-        then
-          self, (Core_models.Option.Option_None <: Core_models.Option.t_Option v_A)
-          <:
-          (t_OnceWith v_F & Core_models.Option.t_Option v_A)
-        else
-          let (tmp0: Rust_primitives.Sequence.t_Seq v_F), (out: v_F) =
-            Rust_primitives.Sequence.seq_remove #v_F self._0 (mk_usize 0)
-          in
-          let self:t_OnceWith v_F = { self with _0 = tmp0 } <: t_OnceWith v_F in
-          self,
-          (Core_models.Option.Option_Some
-            (Core_models.Ops.Function.f_call_once #v_F
-                #Prims.unit
-                #FStar.Tactics.Typeclasses.solve
-                out
-                (() <: Prims.unit))
-            <:
-            Core_models.Option.t_Option v_A)
-          <:
-          (t_OnceWith v_F & Core_models.Option.t_Option v_A)
-      in
-      self, hax_temp_output <: (t_OnceWith v_F & Core_models.Option.t_Option v_A)
-  }
+     = impl' #v_A #v_F #i0 #_
